first attempt at appraisal term generator, trying to leverage evidence shape to prove correctness

Appraisal.v
@@ -1,5 +1,5 @@
-Require Import ConcreteEvidence.
-Require Import Maps OptMonad MonadAM.
+Require Import ConcreteEvidence GenStMonad.
+Require Import Maps (*OptMonad*) MonadAM  StructTact.StructTactics.
 
 Require Import List.
 Import ListNotations.
@@ -37,9 +37,10 @@ Definition check_ev_sig (e:EvidenceC) (k:Pri_Key) (sig:BS) : bool :=
   let payload := encode_ev e in
   check_sig payload k sig.
 
+(*
 Definition check_ev_pl (e:EvidenceC) (p:Plc) (sig:BS) : option bool :=
-  k <- map_get pri_keys p ;;
-    ret (check_ev_sig e k sig).
+  k <- map_get pri_keys p ;; 
+    ret (check_ev_sig e k sig). *)
 
 (* params: payload -> hash *)
 (* TODO: incorporate hash algorithm choice (policy) here? *)
@@ -51,9 +52,10 @@ Definition check_ev_hash (e:EvidenceC) (bs:BS) : bool :=
 
 Check Nat.eqb.
 
+(*
 Definition check_nonce (n : N_ID) (bs:BS) : option bool :=
   g_bs <- map_get nonce_map n ;;
-       ret (Nat.eqb bs g_bs).  
+       ret (Nat.eqb bs g_bs).   
 
 
 Definition check_asp (x:ASP_ID) (m:BS) : option bool :=
@@ -112,6 +114,8 @@ Theorem app_eq_appI: forall e,
     appraise e = run_app il.
 Abort.
 
+
+
 Require Import StVM Instr VmSemantics.
 
 Definition mt_st := mk_st mtc [] [] 0 [].
@@ -123,4 +127,208 @@ Theorem can_app: forall t,
     let optB := run_app app_il in
     exists b, optB = Some b.
 Abort.
+*)
+
+
+
+
+
+(* Specific APP monad state *)
+Definition sig_map := Map Plc ASP_ID.
+Definition hsh_map := Map Plc ASP_ID.
+Definition asp_map := Map (Plc * ASP_ID) ASP_ID.
+Record app_st : Type := mk_app_st
+                         {st_sigmap :sig_map;
+                          st_hshmap :hsh_map; 
+                          st_aspmap :asp_map;
+                          st_nonceCheck_asp :ASP_ID}.
+
+Definition empty_app_st := mk_app_st [] [] [] 0.
+Check empty_app_st.
+
+
+Definition APP := St app_st.
+
+Definition helper_gen_app (a:ASP) (p:Plc) (e:EvidenceC) : APP (Term * EvidenceC) :=
+  match a with
+  | CPY => ret (asp CPY,e)
+  | ASPC i =>
+    match e with
+    | uuc _ bs e' => ret (asp (ASPC 0),e')
+    | _ => failm
+    end
+  | SIG =>
+    match e with
+    | ggc _ _ e' => ret (asp (ASPC 0),e')
+    | _ => failm
+    end
+  | HSH =>
+    match e with
+    | hhc _ e' => ret (asp (ASPC 0),e')
+    | _ => failm
+    end
+  end.
     
+               
+  
+
+Fixpoint gen_appraisal_term' (t:Term) (p:Plc) (e:EvidenceC) : APP (Term * EvidenceC) :=
+  match t with
+  | asp a => helper_gen_app a p e
+  | att q t' => gen_appraisal_term' t' q e
+  | lseq t1 t2 =>
+   (* (t2', e2) *)v2 <- (gen_appraisal_term' t2 p e) ;;
+             (* (t1',e1) *) v1 <- (gen_appraisal_term' t1 p (snd v2)) ;;
+                     ret ((bpar (NONE,NONE) (fst v1) (fst v2)),(snd v1))
+  | bseq _ t1 t2 =>
+      match e with
+      | ssc e1 e2 =>   
+        (* (t1',_) *) v1 <- (gen_appraisal_term' t1 p e1) ;;
+        (* (t2',_) *) v2 <- (gen_appraisal_term' t2 p e2) ;;
+        ret ((bpar (NONE,NONE) (fst v1) (fst v2)),mtc)
+      |_ => failm (* error "evidence mismath on BRS-SS" *)
+      end
+  | bpar _ t1 t2 =>
+      match e with
+      | ppc e1 e2 =>   
+        (* (t1',_) *) v1 <- (gen_appraisal_term' t1 p e1) ;;
+        (* (t2',_) *) v2 <- (gen_appraisal_term' t2 p e2) ;;
+        ret ((bpar (NONE,NONE) (fst v1) (fst v2)),mtc)
+      |_ => failm (* error "evidence mismath on BRP-PP" *)
+      end
+  end.
+
+Require Import Instr MonadVM VmSemantics.
+
+Lemma run_vm_good_ev : forall t tr tr' e e' s s' p p' o o',
+  run_vm (instr_compiler t)
+         {| st_ev := e; st_stack := s;  st_trace := tr; st_pl := p; st_store := o |} =
+  {| st_ev := e'; st_stack := s'; st_trace := tr'; st_pl := p'; st_store := o' |} ->
+  EvcT (unanno t) e e'.
+Proof.
+Admitted.
+
+
+
+    
+
+Theorem someEv : forall t tr tr' e e' s s' p p' o o' app_st,
+  run_vm (instr_compiler t)
+         {| st_ev := e; st_stack := s;  st_trace := tr; st_pl := p; st_store := o |} =
+  {| st_ev := e'; st_stack := s'; st_trace := tr'; st_pl := p'; st_store := o' |} ->
+  exists app_st' v,
+    runSt app_st (gen_appraisal_term' (unanno t) p e') = (Some v,app_st').
+Proof.
+  intros.
+  assert (EvcT (unanno t) e e').
+  eapply run_vm_good_ev; eauto.
+  generalize dependent p.
+  generalize dependent e.
+  generalize dependent e'.
+  generalize dependent tr.
+  generalize dependent tr'.
+  generalize dependent o.
+  generalize dependent o'.
+  generalize dependent s.
+  generalize dependent s'.
+  generalize dependent p'.
+  induction t; intros.
+  - unfold unanno in *.
+    destruct a; simpl; eexists; eexists;
+      try (invc H0; reflexivity).
+  - Print unanno.
+    simpl.
+    eapply IHt.
+    simpl in H0.
+    invc H0.
+    eassumption.
+    admit.
+  - simpl.
+    invc H0.
+    monad_unfold.
+
+    edestruct destruct_compiled_appended.
+    eassumption.
+    destruct H0. destruct H0. destruct H0. destruct H0. destruct H0.
+
+    destruct H1. destruct H1.
+     assert (EvcT (unanno t2) x0 e'). {
+       eapply run_vm_good_ev. eauto. }
+
+     edestruct IHt2.
+     apply H4.
+     apply H1.
+     destruct H5.
+     assert (p = x2). admit.
+     rewrite H7.
+     rewrite H5.
+
+
+    
+    assert (EvcT (unanno t1) e x0). {
+      eapply run_vm_good_ev; eauto. }
+
+    edestruct IHt1.
+    apply H8.
+    eassumption.
+
+    destruct H9.
+    destruct x6.
+    destruct x8.
+    simpl.
+    rewrite <- H7.
+
+    assert (x0 = e0). admit. (* Interesting symmetry:  t1(e) = x0, gen_app_term t2(e') = e0 *)
+    assert (app_st0 = x5). admit. (* TODO: st immutable *)
+
+    rewrite <- H10.
+    rewrite <- H11.
+    rewrite H9.
+    eexists. eexists. reflexivity.
+  - simpl.
+    invc H0.
+    monad_unfold.
+
+    unfold run_vm_step in H.
+    simpl in H.
+    monad_unfold.
+    
+    edestruct destruct_compiled_appended.
+    eassumption.
+    destruct H0. destruct H0. destruct H0. destruct H0. destruct H0.
+
+    destruct H1. destruct H1.
+
+    do_run.
+    monad_unfold.
+    simpl in H4.
+    monad_unfold.
+    unfold pop_stackm in H4.
+    monad_unfold.
+    simpl in H4.
+
+    edestruct destruct_compiled_appended.
+    eapply H4.
+
+
+
+    
+     assert (EvcT (unanno t2) x0 e'). {
+       eapply run_vm_good_ev; eauto. }
+
+     edestruct IHt2.
+     apply H7.
+     apply H1.
+     destruct H8.
+     destruct H4.
+
+      
+      
+
+
+      }
+    eassumption.
+    admit.
+    
+  
+  
